

ياد محمد خالد عبد الفتاح ; Bonus 3: $\int_{-1}^1 P_n(x) P_n(x) dx = \frac{2}{2n+1}$

use generating function

$$\frac{1}{\sqrt{1-2xt+t^2}} = \sum_{n=0}^{\infty} P_n(x) t^n$$

multiply by generating function again (but in sigma notation in R.H.S)

$$\frac{1}{1-2xt+t^2} = \sum_{n=0}^{\infty} \sum_{m=0}^{\infty} P_n(x) P_m(x) t^{n+m}$$

now integrate both sides from -1 to 1 with respect to x

$$\int_{-1}^1 \frac{1}{1-2xt+t^2} dx = \sum_{n=0}^{\infty} \sum_{m=0}^{\infty} t^{n+m} \int_{-1}^1 P_n(x) P_m(x) dx$$

use orthogonality: $\int_{-1}^1 P_n(x) P_m(x) dx = 0$ where $m \neq n$

$$\int_{-1}^1 \frac{1}{1-2xt+t^2} dx = \sum_{n=0}^{\infty} t^{2n} \int_{-1}^1 [P_n(x)]^2 dx$$

$$\begin{aligned} \text{L.H.S} &= \int_{-1}^1 \frac{1}{1-2xt+t^2} dx = \int_{-1}^1 \frac{1}{(1+t^2)-2xt} dx = \frac{1}{-2t} \int_{-1}^1 \frac{-2t}{(1+t^2)-2xt} dx \\ &= \frac{-1}{2t} \left[\ln(1-2xt+t^2) \right]_{-1}^1 = \frac{-1}{2t} \left[\ln(1-t^2) - \ln(1+t^2) \right] \\ &= \frac{-1}{2t} \left[2 \ln(1-t) - 2 \ln(1+t) \right] = \frac{-1}{t} \left[\ln(1-t) - \ln(1+t) \right] \end{aligned}$$